P4cub: decidable type equivalence, header stack values have type information

deps/coq-poulet4/lib/P4cub/AST.v
@@ -2,6 +2,8 @@ Require Export Coq.Lists.List.
 Export ListNotations.
 Require Export Coq.Bool.Bool.
 Require Export P4cub.Utiliser.
+Require Import Coq.PArith.BinPosDef.
+Require Import Coq.PArith.BinPos.
 
 (** Notation entries. *)
 Declare Custom Entry p4type.
@@ -311,6 +313,29 @@ Module P4cub.
 
         Import TypeNotations.
 
+        (** Decidable equality. *)
+        Fixpoint eqbt (τ1 τ2 : t tags_t) : bool :=
+          let fix frec (ts1 ts2 : F.fs tags_t (t tags_t)) : bool :=
+              match ts1, ts2 with
+              | [], [] => true
+              | (x1,t1)::ts1, (x2,t2)::ts2 => if P4String.equivb x1 x2 then
+                                             eqbt t1 t2 && frec ts1 ts2
+                                           else false
+              | [], _::_ | _::_, [] => false
+              end in
+          match τ1, τ2 with
+          | {{ Bool }}, {{ Bool }}
+          | {{ error }}, {{ error }}
+          | {{ matchkind }}, {{ matchkind }} => true
+          | {{ bit<w1> }}, {{ bit<w2> }}
+          | {{ int<w1> }}, {{ int<w2> }} => (w1 =? w2)%positive
+          | {{ hdr { ts1 } }}, {{ hdr { ts2 } }}
+          | {{ rec { ts1 } }}, {{ rec { ts2 } }} => frec ts1 ts2
+          | {{ stack ts1[n1] }}, {{ stack ts2[n2] }} => (n1 =? n2)%positive && frec ts1 ts2
+          | _, _ => false
+          end.
+        (**[]*)
+
         (** Equality of types. *)
         Inductive equivt : t tags_t -> t tags_t -> Prop :=
         | equivt_bool : ∫ Bool ≡ Bool
@@ -439,41 +464,62 @@ Module P4cub.
                        | apply equivt_transitive].
         Defined.
 
-        Lemma equivt_dec : forall (t1 t2 : t tags_t),
-            equivt t1 t2 \/ ~ equivt t1 t2.
+        Lemma equivt_eqbt : forall t1 t2, equivt t1 t2 -> eqbt t1 t2 = true.
         Proof.
-          induction t1 using custom_t_ind; intros [];
-            try (left; apply equivt_reflexive);
-            try (right; intros HR; inversion HR; assumption);
-            try (destruct (equiv_dec w width) as [Hwidth | Hwidth];
-                 unfold equiv in *; unfold complement in *; subst;
-                 try (right; intros H'; inversion H'; contradiction);
-                 try (left; reflexivity));
-            try (destruct (equiv_dec size size0) as [Hsize | Hsize];
-                 unfold equiv in *; unfold complement in *; subst;
-                 try (right; intros H'; inversion H'; contradiction));
+          intros t1 t2 H.
+          induction H using custom_equivt_ind;
+            simpl in *; try rewrite Pos.eqb_refl; auto;
+              rename H0 into HR;
+              try (induction H; inv HR; auto;
+                   destruct x as [x1 t1]; destruct y as [x2 t2];
+                     simpl in *; repeat invert_relf; simpl in *;
+                       pose proof P4String.equiv_reflect x1 x2 as Hx;
+                       inv Hx; try contradiction; rewrite H2; auto).
+          Qed.
+
+        Lemma eqbt_equivt : forall t1 t2, eqbt t1 t2 = true -> equivt t1 t2.
+        Proof.
+          induction t1 using custom_t_ind; intros [] Heqbt; simpl in *;
+            try apply andb_true_iff in Heqbt as [Hpos Heqbt];
+            try discriminate;
+            try match goal with
+                | H: (_ =? _)%positive = true |- _ => apply Peqb_true_eq in H; subst
+                end;
+            constructor;
             try (rename fields into fs1; rename fields0 into fs2;
                  generalize dependent fs2;
-                 induction fs1 as [| [x1 t1] fs1 IHfs1];
-                 intros [| [x2 t2] fs2];
-                 try (left; reflexivity);
-                 try (right; intros H';
-                      inversion H'; try invert_nil_cons_relate; assumption); subst;
-                 inversion H; clear H; subst; unfold F.predf_data in *;
-                 pose proof IHfs1 H3 fs2 as IH; clear IHfs1 H3;
-                 destruct (equiv_dec x1 x2) as [H12 | H12];
-                 unfold equiv in *; unfold complement in *;
-                 destruct (H2 t2) as [HT | HT]; clear H2;
-                 destruct IH as [IH | IH];
-                 try (right; intros H'; inversion H';
-                      clear H'; subst; invert_cons_cons_relate;
-                      subst; unfold F.relf in *;
-                      simpl in *; destruct H3; contradiction);
-                 [ left; constructor; inversion IH; subst;
-                   constructor; auto; unfold F.relf; split; auto
-                 | right; intros H'; inversion H'; subst;
-                   clear H'; invert_cons_cons_relate; subst; apply IH;
-                   constructor; auto ]).
+                   induction fs1 as [| [x1 t1] fs1 IHfs1];
+                   intros [| [x2 t2] fs2] IH; inv H; simpl in *;
+                     try discriminate; constructor;
+                       destruct (P4String.equivb x1 x2) eqn:Hx;
+                       destruct (eqbt t1 t2) eqn:Heqbt;
+                       try discriminate; simpl in *;
+                         [ split; simpl; auto;
+                           pose proof P4String.equiv_reflect x1 x2 as Hx';
+                           inv Hx'; try contradiction; auto;
+                           rewrite Hx in H; discriminate
+                         | apply IHfs1; auto ]).
+          Qed.
+
+        Lemma equivt_eqbt_iff : forall t1 t2 : t tags_t, equivt t1 t2 <-> eqbt t1 t2 = true.
+        Proof.
+          intros t1 t2; split; [apply equivt_eqbt | apply eqbt_equivt].
+        Qed.
+
+        Lemma equivt_reflect : forall t1 t2, reflect (equivt t1 t2) (eqbt t1 t2).
+        Proof.
+          intros t1 t2.
+          destruct (eqbt t1 t2) eqn:Heqbt; constructor.
+          - apply eqbt_equivt; assumption.
+          - intros H. apply equivt_eqbt in H.
+            rewrite H in Heqbt. discriminate.
+        Qed.
+
+        Lemma equivt_dec : forall t1 t2 : t tags_t,
+            equivt t1 t2 \/ ~ equivt t1 t2.
+        Proof.
+          intros t1 t2. pose proof equivt_reflect t1 t2 as H.
+          inversion H; subst; auto.
         Qed.
       End TypeEquivalence.
     End TypeEquivalence.
